Add keyring trace (#48)
* Add keyring trace

* Add stricter postconditions for keyring traces for OnEncrypt/OnDecrypt

* Add conditions on materials and keyring trait

* Move non-stateful requirements of materials to keyrings

* Fix HKDF verification timeout

* Add functional tests for keyrings and fix RawAESKeyring implementation

src/SDK/Materials.dfy
@@ -3,7 +3,6 @@ include "../StandardLibrary/UInt.dfy"
 include "./AlgorithmSuite.dfy"
 include "../Util/UTF8.dfy"
 
-
 module Materials {
   import opened StandardLibrary
   import opened UInt = StandardLibrary.UInt
@@ -19,9 +18,9 @@ module Materials {
   const EC_PUBLIC_KEY_FIELD := UTF8.Encode("aws-crypto-public-key").value
   ghost const ReservedKeyValues := { EC_PUBLIC_KEY_FIELD }
 
-  datatype EncryptedDataKey = EncryptedDataKey(providerID : UTF8.ValidUTF8Bytes,
-                                               providerInfo : seq<uint8>,
-                                               ciphertext : seq<uint8>)
+  datatype EncryptedDataKey = EncryptedDataKey(providerID: UTF8.ValidUTF8Bytes,
+                                               providerInfo: seq<uint8>,
+                                               ciphertext: seq<uint8>)
   {
     predicate Valid() {
       |providerID| < UINT16_LIMIT &&
@@ -36,37 +35,98 @@ module Materials {
 
   type ValidEncryptedDataKey = i : EncryptedDataKey | i.Valid() witness EncryptedDataKey.ValidWitness()
 
-  // TODO: Add keyring trace
+  datatype KeyringTraceFlag =
+  | GENERATED_DATA_KEY
+  | ENCRYPTED_DATA_KEY
+  | DECRYPTED_DATA_KEY
+  | SIGNED_ENCRYPTION_CONTEXT
+  | VERIFIED_ENCRYPTION_CONTEXT
+
+  datatype KeyringTraceEntry = KeyringTraceEntry(keyNamespace: UTF8.ValidUTF8Bytes,
+                                                 keyName: UTF8.ValidUTF8Bytes,
+                                                 flags: set<KeyringTraceFlag>)
+
+  predicate method IsGenerateTraceEntry(entry: KeyringTraceEntry) {
+    GENERATED_DATA_KEY in entry.flags
+  }
+
+  predicate method IsEncryptTraceEntry(entry: KeyringTraceEntry) {
+    ENCRYPTED_DATA_KEY in entry.flags
+  }
+
+  predicate method IsDecryptTraceEntry(entry: KeyringTraceEntry) {
+    DECRYPTED_DATA_KEY in entry.flags
+  }
+
+  const ValidEncryptionMaterialFlags: set<KeyringTraceFlag> := {ENCRYPTED_DATA_KEY, SIGNED_ENCRYPTION_CONTEXT, GENERATED_DATA_KEY};
+  const ValidDecryptionMaterialFlags: set<KeyringTraceFlag> := {DECRYPTED_DATA_KEY, VERIFIED_ENCRYPTION_CONTEXT};
+
   datatype DataKeyMaterials = DataKeyMaterials(algorithmSuiteID: AlgorithmSuite.ID,
                                                plaintextDataKey: seq<uint8>,
-                                               encryptedDataKeys: seq<ValidEncryptedDataKey>) 
+                                               encryptedDataKeys: seq<ValidEncryptedDataKey>,
+                                               keyringTrace: seq<KeyringTraceEntry>)
   {
     predicate method Valid() {
-      algorithmSuiteID.ValidPlaintextDataKey(plaintextDataKey)
+      var generateTraces := Filter(keyringTrace, IsGenerateTraceEntry);
+      var encryptTraces := Filter(keyringTrace, IsEncryptTraceEntry);
+      && algorithmSuiteID.ValidPlaintextDataKey(plaintextDataKey)
+      && (forall entry :: entry in keyringTrace ==> entry.flags <= ValidEncryptionMaterialFlags)
+      && (forall entry :: entry in keyringTrace ==> IsGenerateTraceEntry(entry) || IsEncryptTraceEntry(entry))
+      && |generateTraces| <= 1
+      && (|generateTraces| == 1 ==> keyringTrace[0] == generateTraces[0])
+      && |encryptTraces| == |encryptedDataKeys|
+      // TODO: Strongly tie each trace entry to it's corresponding EDK (https://github.com/awslabs/aws-encryption-sdk-dafny/issues/100)
     }
 
-    static function method ValidWitness(): DataKeyMaterials { 
-      DataKeyMaterials(AlgorithmSuite.AES_256_GCM_IV12_TAG16_HKDF_SHA384_ECDSA_P384, 
-                      seq(32, i => 0), 
-                      [EncryptedDataKey.ValidWitness()])
+    static function method ValidWitness(): DataKeyMaterials {
+      DataKeyMaterials(AlgorithmSuite.AES_256_GCM_IV12_TAG16_HKDF_SHA384_ECDSA_P384,
+                      seq(32, i => 0),
+                      [EncryptedDataKey.ValidWitness()],
+                      [KeyringTraceEntry([], [], {ENCRYPTED_DATA_KEY, GENERATED_DATA_KEY})])
     }
   }
 
   type ValidDataKeyMaterials = i: DataKeyMaterials | i.Valid() witness DataKeyMaterials.ValidWitness()
 
   predicate method CompatibleDataKeyMaterials(k1: ValidDataKeyMaterials, k2: ValidDataKeyMaterials) {
+    var generateTraces := Filter(k1.keyringTrace + k2.keyringTrace, IsGenerateTraceEntry);
     k1.algorithmSuiteID == k2.algorithmSuiteID && k1.plaintextDataKey == k2.plaintextDataKey
+    && |generateTraces| <= 1
+    && (|generateTraces| == 1 ==> |k1.keyringTrace| > 0 && generateTraces[0] == k1.keyringTrace[0])
   }
 
-  function method MergeDataKeyMaterials(k1: ValidDataKeyMaterials, k2: ValidDataKeyMaterials): (res: ValidDataKeyMaterials)
+  function method ConcatDataKeyMaterials(k1: ValidDataKeyMaterials, k2: ValidDataKeyMaterials): (res: ValidDataKeyMaterials)
     requires CompatibleDataKeyMaterials(k1, k2)
     ensures res.algorithmSuiteID == k1.algorithmSuiteID == k2.algorithmSuiteID
     ensures res.plaintextDataKey == k1.plaintextDataKey == k2.plaintextDataKey
     ensures res.encryptedDataKeys == k1.encryptedDataKeys + k2.encryptedDataKeys
+    ensures res.keyringTrace == k1.keyringTrace + k2.keyringTrace
   {
-    var r := DataKeyMaterials(k1.algorithmSuiteID, k1.plaintextDataKey, k1.encryptedDataKeys + k2.encryptedDataKeys);
+    FilterIsDistributive(k1.keyringTrace, k2.keyringTrace, IsEncryptTraceEntry);
+    FilterIsDistributive(k1.keyringTrace, k2.keyringTrace, IsGenerateTraceEntry);
+    var r := DataKeyMaterials(k1.algorithmSuiteID, k1.plaintextDataKey, k1.encryptedDataKeys + k2.encryptedDataKeys, k1.keyringTrace + k2.keyringTrace);
     r
   }
+
+  datatype OnDecryptResult = OnDecryptResult(algorithmSuiteID: AlgorithmSuite.ID,
+                                             plaintextDataKey: seq<uint8>,
+                                             keyringTrace: seq<KeyringTraceEntry>)
+  {
+    predicate Valid() {
+      && algorithmSuiteID.ValidPlaintextDataKey(plaintextDataKey)
+      && (forall entry :: entry in keyringTrace ==> entry.flags <= ValidDecryptionMaterialFlags)
+    }
+
+    static function method ValidWitness(): OnDecryptResult {
+      var pdk := seq(32, i => 0);
+      var entry := KeyringTraceEntry([], [], {DECRYPTED_DATA_KEY});
+      var r := OnDecryptResult(AlgorithmSuite.AES_256_GCM_IV12_TAG16_HKDF_SHA384_ECDSA_P384,
+                      pdk, [entry]);
+      r
+    }
+  }
+
+  type ValidOnDecryptResult = i: OnDecryptResult | i.Valid() witness OnDecryptResult.ValidWitness()
 
   datatype EncryptionMaterials = EncryptionMaterials(encryptionContext: EncryptionContext,
                                                      dataKeyMaterials: ValidDataKeyMaterials,
@@ -77,28 +137,33 @@ module Materials {
       && |dataKeyMaterials.encryptedDataKeys| > 0
     }
 
-    static function method ValidWitness(): EncryptionMaterials { 
-       EncryptionMaterials([], DataKeyMaterials.ValidWitness(), Some(seq(32, i => 0)))
+    static function method ValidWitness(): EncryptionMaterials {
+      EncryptionMaterials([], DataKeyMaterials.ValidWitness(), Some(seq(32, i => 0)))
     }
   }
+
   type ValidEncryptionMaterials = i: EncryptionMaterials | i.Valid() witness EncryptionMaterials.ValidWitness()
 
-  // TODO: Add keyring trace
   datatype DecryptionMaterials = DecryptionMaterials(algorithmSuiteID: AlgorithmSuite.ID,
                                                      encryptionContext: EncryptionContext,
                                                      plaintextDataKey: seq<uint8>,
-                                                     verificationKey: Option<seq<uint8>>)
+                                                     verificationKey: Option<seq<uint8>>,
+                                                     keyringTrace: seq<KeyringTraceEntry>)
+
   {
     predicate method Valid() {
       && algorithmSuiteID.ValidPlaintextDataKey(plaintextDataKey)
       && algorithmSuiteID.SignatureType().Some? ==> verificationKey.Some?
+      && (forall entry :: entry in keyringTrace ==> entry.flags <= ValidDecryptionMaterialFlags)
     }
 
-    static function method ValidWitness(): DecryptionMaterials { 
+    static function method ValidWitness(): DecryptionMaterials {
       DecryptionMaterials(AlgorithmSuite.AES_256_GCM_IV12_TAG16_HKDF_SHA384_ECDSA_P384,
-                          [], seq(32, i => 0), Some(seq(32, i => 0)))
+                          [], seq(32, i => 0), Some(seq(32, i => 0)),
+                          [KeyringTraceEntry([], [], {DECRYPTED_DATA_KEY})])
     }
   }
+
   type ValidDecryptionMaterials = i: DecryptionMaterials | i.Valid() witness DecryptionMaterials.ValidWitness()
 
     //TODO: Review this code.
